CoqOfRust/ink/ink_engine.v
@@ -304,6 +304,64 @@ Module DebugInfo.
 End DebugInfo.
 Definition DebugInfo : Set := @DebugInfo.t.
 
+Module chain_extension.
+  Module ChainExtensionHandler.
+    Unset Primitive Projections.
+    Record t : Set := {
+      registered
+        :
+        std.collections.hash.map.HashMap
+          ink_engine.chain_extension.ExtensionId
+          (alloc.boxed.Box TraitObject);
+      output : alloc.vec.Vec u8;
+    }.
+    Global Set Primitive Projections.
+    
+    Global Instance Get_registered : Notation.Dot "registered" := {
+      Notation.dot '(Build_t x0 _) := x0;
+    }.
+    Global Instance Get_output : Notation.Dot "output" := {
+      Notation.dot '(Build_t _ x1) := x1;
+    }.
+  End ChainExtensionHandler.
+  Definition ChainExtensionHandler : Set := @ChainExtensionHandler.t.
+  
+  Module ExtensionId.
+    Unset Primitive Projections.
+    Record t : Set := {
+      _ : u32;
+    }.
+    Global Set Primitive Projections.
+    
+    Global Instance Get_0 : Notation.Dot 0 := {
+      Notation.dot '(Build_t x0) := x0;
+    }.
+  End ExtensionId.
+  Definition ExtensionId := @ExtensionId.t.
+  
+  Module ChainExtension.
+    Class Trait (Self : Set) : Set := {
+      func_id `{H : State.Trait} : (ref Self) -> (M (H := H) u32);
+      call
+        `{H : State.Trait}
+        :
+        (mut_ref Self) ->
+        (ref (Slice u8)) ->
+        (mut_ref (alloc.vec.Vec u8)) ->
+        (M (H := H) u32);
+    }.
+    
+    Global Instance Method_func_id `{H : State.Trait} `(Trait)
+      : Notation.Dot "func_id" := {
+      Notation.dot := func_id;
+    }.
+    Global Instance Method_call `{H : State.Trait} `(Trait)
+      : Notation.Dot "call" := {
+      Notation.dot := call;
+    }.
+  End ChainExtension.
+End chain_extension.
+
 Module ChainExtensionHandler.
   Unset Primitive Projections.
   Record t : Set := {
@@ -360,6 +418,32 @@ Module ChainExtension.
   }.
 End ChainExtension.
 
+Module database.
+  Parameter balance_of_key : forall `{H : State.Trait},
+      ref (Slice u8) ->
+      M (H := H) list u8.
+  
+  Parameter storage_of_contract_key : forall `{H : State.Trait},
+      ref (Slice u8) ->
+      ref (Slice u8) ->
+      M (H := H) list u8.
+  
+  Module Database.
+    Unset Primitive Projections.
+    Record t : Set := {
+      hmap
+        :
+        std.collections.hash.map.HashMap (alloc.vec.Vec u8) (alloc.vec.Vec u8);
+    }.
+    Global Set Primitive Projections.
+    
+    Global Instance Get_hmap : Notation.Dot "hmap" := {
+      Notation.dot '(Build_t x0) := x0;
+    }.
+  End Database.
+  Definition Database : Set := @Database.t.
+End database.
+
 Parameter balance_of_key : forall `{H : State.Trait},
     ref (Slice u8) ->
     M (H := H) list u8.
@@ -383,6 +467,42 @@ Module Database.
   }.
 End Database.
 Definition Database : Set := @Database.t.
+
+Module exec_context.
+  Module ExecContext.
+    Unset Primitive Projections.
+    Record t : Set := {
+      caller : core.option.Option ink_engine.types.AccountId;
+      callee : core.option.Option ink_engine.types.AccountId;
+      value_transferred : ink_engine.types.Balance;
+      block_number : ink_engine.types.BlockNumber;
+      block_timestamp : ink_engine.types.BlockTimestamp;
+      contracts : alloc.vec.Vec (alloc.vec.Vec u8);
+    }.
+    Global Set Primitive Projections.
+    
+    Global Instance Get_caller : Notation.Dot "caller" := {
+      Notation.dot '(Build_t x0 _ _ _ _ _) := x0;
+    }.
+    Global Instance Get_callee : Notation.Dot "callee" := {
+      Notation.dot '(Build_t _ x1 _ _ _ _) := x1;
+    }.
+    Global Instance Get_value_transferred :
+        Notation.Dot "value_transferred" := {
+      Notation.dot '(Build_t _ _ x2 _ _ _) := x2;
+    }.
+    Global Instance Get_block_number : Notation.Dot "block_number" := {
+      Notation.dot '(Build_t _ _ _ x3 _ _) := x3;
+    }.
+    Global Instance Get_block_timestamp : Notation.Dot "block_timestamp" := {
+      Notation.dot '(Build_t _ _ _ _ x4 _) := x4;
+    }.
+    Global Instance Get_contracts : Notation.Dot "contracts" := {
+      Notation.dot '(Build_t _ _ _ _ _ x5) := x5;
+    }.
+  End ExecContext.
+  Definition ExecContext : Set := @ExecContext.t.
+End exec_context.
 
 Module ExecContext.
   Unset Primitive Projections.
@@ -417,6 +537,28 @@ Module ExecContext.
 End ExecContext.
 Definition ExecContext : Set := @ExecContext.t.
 
+Module hashing.
+  Parameter blake2b_256 : forall `{H : State.Trait},
+      ref (Slice u8) ->
+      mut_ref list u8 ->
+      M (H := H) unit.
+  
+  Parameter blake2b_128 : forall `{H : State.Trait},
+      ref (Slice u8) ->
+      mut_ref list u8 ->
+      M (H := H) unit.
+  
+  Parameter keccak_256 : forall `{H : State.Trait},
+      ref (Slice u8) ->
+      mut_ref list u8 ->
+      M (H := H) unit.
+  
+  Parameter sha2_256 : forall `{H : State.Trait},
+      ref (Slice u8) ->
+      mut_ref list u8 ->
+      M (H := H) unit.
+End hashing.
+
 Parameter blake2b_256 : forall `{H : State.Trait},
     ref (Slice u8) ->
     mut_ref list u8 ->
@@ -436,6 +578,48 @@ Parameter sha2_256 : forall `{H : State.Trait},
     ref (Slice u8) ->
     mut_ref list u8 ->
     M (H := H) unit.
+
+Module types.
+  Definition BlockNumber : Set := u32.
+  
+  Definition BlockTimestamp : Set := u64.
+  
+  Definition Balance : Set := u128.
+  
+  Module AccountId.
+    Unset Primitive Projections.
+    Record t : Set := {
+      _ : alloc.vec.Vec u8;
+    }.
+    Global Set Primitive Projections.
+    
+    Global Instance Get_0 : Notation.Dot 0 := {
+      Notation.dot '(Build_t x0) := x0;
+    }.
+  End AccountId.
+  Definition AccountId := @AccountId.t.
+  
+  Module Key.
+    Unset Primitive Projections.
+    Record t : Set := {
+      _ : alloc.vec.Vec u8;
+    }.
+    Global Set Primitive Projections.
+    
+    Global Instance Get_0 : Notation.Dot 0 := {
+      Notation.dot '(Build_t x0) := x0;
+    }.
+  End Key.
+  Definition Key := @Key.t.
+  
+  Module AccountError.
+    Inductive t : Set :=
+    | Decoding (_ : parity_scale_codec.error.Error)
+    | UnexpectedUserAccount
+    | NoAccountForId (_ : alloc.vec.Vec u8).
+  End AccountError.
+  Definition AccountError := AccountError.t.
+End types.
 
 Definition BlockNumber : Set := u32.
 
