coq_translation/axiomatized/examples/testing/unit_testing.v
@@ -2,3 +2,7 @@
 Require Import CoqOfRust.CoqOfRust.
 
 Parameter add : forall `{H : State.Trait}, i32 -> i32 -> M (H := H) i32.
+
+Module tests.
+  
+End tests.
